code/ecdsa/Hacl.Impl.EC.General.PointDouble.fsti
@@ -1,4 +1,4 @@
-module Hacl.Impl.EC.PointDouble
+module Hacl.Impl.EC.General.PointDouble
 
 open FStar.HyperStack.All
 open FStar.HyperStack
@@ -14,12 +14,6 @@ open Spec.ECC.Curves
 
 open Hacl.Spec.MontgomeryMultiplication
 
-open Hacl.Impl.EC.K.PointDouble
-open Hacl.Impl.EC.General.PointDouble
-open Hacl.Impl.EC.NIST.PointDouble
-
-
-
 
 #set-options "--z3rlimit 300 --ifuel 0 --fuel 0" 
 
@@ -32,12 +26,4 @@ val point_double: #c: curve -> p: point c -> result: point c
     disjoint p tempBuffer /\ disjoint result tempBuffer /\
     eq_or_disjoint p result /\ point_eval c h p)
   (ensures fun h0 _ h1 -> modifies (loc tempBuffer |+| loc result) h0 h1 /\ point_eval c h1 result /\ (      
-    fromDomainPoint #c #DH (point_as_nat c h1 result) == _point_double #c (fromDomainPoint #c #DH (point_as_nat c h0 p))))
-
-
-let point_double #c p result =
-  match c with 
-  |P256 -> Hacl.Impl.EC.NIST.PointDouble.point_double #P256 p result
-  |P384 -> Hacl.Impl.EC.NIST.PointDouble.point_double #P384 p result
-  |Default -> Hacl.Impl.EC.NIST.PointDouble.point_double #Default p result
-
+    fromDomainPoint #c #DH (point_as_nat c h1 result) == _point_double_general #c (fromDomainPoint #c #DH (point_as_nat c h0 p))))
