specs/ecdsap256/Spec.ECC.fst
@@ -23,7 +23,7 @@ let isPointAtInfinity (p:point_nat) =
   let (_, _, z) = p in z = 0
 
 noextract
-let _point_double #curve (p:point_nat_prime #curve) : point_nat_prime #curve =
+let _point_double_nist #curve (p:point_nat_prime #curve) : point_nat_prime #curve =
   let prime = getPrime curve in 
   let x, y, z = p in
   let delta = z * z in 
@@ -34,6 +34,49 @@ let _point_double #curve (p:point_nat_prime #curve) : point_nat_prime #curve =
   let y3 = (alpha * (4 * beta - x3) - 8 * gamma * gamma) % prime in 
   let z3 = ((y + z) * (y + z) - delta - gamma) % prime in 
   (x3, y3, z3)
+
+
+(* https://www.hyperelliptic.org/EFD/g1p/auto-shortw-jacobian.html#doubling-dbl-1998-cmo-2 *)
+
+noextract
+let _point_double_general #curve (p: point_nat_prime #curve) : point_nat_prime #curve = 
+  let prime = getPrime curve in 
+  let x, y, z = p in
+  let gamma = y * y in 
+  let delta = z * z in 
+  let beta = x * gamma in 
+   
+  let alpha = 3 * x * x + aCoordinate #curve * delta * delta in 
+  
+  let x3 = (alpha * alpha - 8 * beta) % prime in 
+  let y3 = (alpha * (4 * beta - x3) - 8 * gamma * gamma) % prime in 
+  let z3 = ((y + z) * (y + z) - delta - gamma) % prime in 
+  (x3, y3, z3)
+
+
+noextract
+let _point_double_koblitz #curve (p: point_nat_prime #curve) : point_nat_prime #curve = 
+  let prime = getPrime curve in 
+  let x, y, z = p in
+  let gamma = y * y in 
+  let delta = z * z in 
+  let beta = x * gamma in 
+   
+  let alpha = 3 * x * x in 
+  
+  let x3 = (alpha * alpha - 8 * beta) % prime in 
+  let y3 = (alpha * (4 * beta - x3) - 8 * gamma * gamma) % prime in 
+  let z3 = ((y + z) * (y + z) - delta - gamma) % prime in 
+  (x3, y3, z3)
+
+
+noextract
+let _point_double #curve (p: point_nat_prime) : point_nat_prime #curve = 
+  match curve with 
+  |P256 -> _point_double_nist p 
+  |P384 -> _point_double_nist p
+  |Default -> _point_double_general p
+
 
 
  let _norm #curve (p:point_nat_prime #curve) : (point_nat_prime #curve) =
@@ -119,7 +162,7 @@ let _point_add #curve (p:point_nat_prime #curve) (q:point_nat_prime #curve) : po
 
 let pointAdd #curve (p:point_nat_prime #curve) (q:point_nat_prime #curve) : point_nat_prime #curve =
   if pointEqual p q then 
-    _point_double p 
+    _point_double_nist p 
   else
     _point_add p q
 
